corrected the solution for (a) and (b)

1.dfy
@@ -4,43 +4,34 @@
 /*_________________________________________________________________________________________________________*/
 
 
-/**
-(a)
-Define a Dafny specification function called sum that takes as arguments an array of in-
-tegers a and two indices into the array, i and j, that calculates the sum over the interval
-[ai, aj[, with i ≤ j. This function will recur over the array either “from the start” (i.e.,
-recursive calls increase the argument i), or “from the end” (i.e., recursive calls decrease
-the argument j). Note: You will need to add to the function signature a specification of
-the form reads a, to indicate that the function can read from the memory denoted by the
-array. You will also likely reduce future pain if you constrain (i.e., require) i and j such
-that both sum(a,a.Length,a.Length) and sum(a,0,0) are valid function calls.
-*/
 
-function sumFowards(a: array<int>, i: int, j: int): int
+//(a)
+function sum(a: array<int>, i: int, j: int): int
     reads a
     requires 0 <= i <= j <= a.Length
     decreases j - i
 {
     if (i == j) then 0
-    else a[i] + sumFowards(a, i+1, j)
+    else a[i] + sum(a, i+1, j)
 }
 
-method sum(a: array<int>, i: int, j: int) returns (sum:int)
+
+//(b)
+method query(a: array<int>, i: int, j: int) returns (res:int)
     requires 0 <= i <= j <= a.Length
-    ensures sum == sumFowards(a, i, j)
+    ensures res == sum(a, i, j)
 {
-    sum := 0;
+    res := 0;
     var k := i;
 
     while(k < j)
         invariant i <= k <= j <= a.Length
-        invariant sum + sumFowards(a, k, j)  == sumFowards(a, i, j)
+        invariant res + sum(a, k, j)  == sum(a, i, j)
     {
-        sum := sum + a[k];
+        res := res + a[k];
         k := k + 1;
     }
     
 }
 
 
-/*_________________________________________________________________________________________________________*/
